feat: add minimal support for `getEntry`/`getEntry?`/`getEntry!`/`getEntryD` for DHashMap (#11076)
This PR adds `getEntry`/`getEntry?`/`getEntry!`/`getEntryD` operation on
DHashMap.

src/Std/Data/DHashMap/Basic.lean
@@ -190,6 +190,18 @@ end
 @[inline, inherit_doc Raw.getKeyD] def getKeyD (m : DHashMap α β) (a : α) (fallback : α) : α :=
   Raw₀.getKeyD ⟨m.1, m.2.size_buckets_pos⟩ a fallback
 
+@[inline, inherit_doc Raw.getEntry?] def getEntry? (m : DHashMap α β) (a : α) : Option ((a : α) × β a) :=
+  Raw₀.getEntry? ⟨m.1, m.2.size_buckets_pos⟩ a
+
+@[inline, inherit_doc Raw.getEntry] def getEntry (m : DHashMap α β) (a : α) (h : a ∈ m) : (a : α) × β a :=
+  Raw₀.getEntry ⟨m.1, m.2.size_buckets_pos⟩ a h
+
+@[inline, inherit_doc Raw.getEntry!] def getEntry! [Inhabited ((a : α) × β a)] (m : DHashMap α β) (a : α) : (a : α) × β a :=
+  Raw₀.getEntry! ⟨m.1, m.2.size_buckets_pos⟩ a
+
+@[inline, inherit_doc Raw.getEntryD] def getEntryD (m : DHashMap α β) (a : α) (fallback : (a : α) × β a) : (a : α) × β a :=
+  Raw₀.getEntryD ⟨m.1, m.2.size_buckets_pos⟩ a fallback
+
 @[inline, inherit_doc Raw.size] def size (m : DHashMap α β) : Nat :=
   m.1.size
 
