src/Std/Data/Internal/List/Associative.lean
@@ -49,8 +49,25 @@ def getEntry? [BEq α] (a : α) : List ((a : α) × β a) → Option ((a : α) �
   | [] => none
   | ⟨k, v⟩ :: l => bif k == a then some ⟨k, v⟩ else getEntry? a l
 
+/-- Internal implementation detail of the hash map -/
+def getEntryD [BEq α] (a : α) (fallback : (a : α) × β a) : List ((a : α) × β a) → (a : α) × β a
+  | [] => fallback
+  | ⟨k, v⟩ :: l => bif k == a then ⟨k, v⟩ else getEntryD a fallback l
+
+/-- Internal implementation detail of the hash map -/
+def getEntry! [BEq α] (a : α) [Inhabited ((a : α) × β a)] : List ((a : α) × β a) → (a : α) × β a
+  | [] => panic! "key is not present in associative list"
+  | ⟨k, v⟩ :: l => bif k == a then ⟨k, v⟩ else getEntry! a l
+
 @[simp] theorem getEntry?_nil [BEq α] {a : α} :
     getEntry? a ([] : List ((a : α) × β a)) = none := (rfl)
+
+@[simp] theorem getEntryD_nil [BEq α] {a : α} (fallback : (a : α) × β a) :
+    getEntryD a fallback ([] : List ((a : α) × β a)) = fallback := (rfl)
+
+@[simp] theorem getEntry!_nil [BEq α] {a : α} [Inhabited ((a : α) × β a)] :
+    getEntry! a ([] : List ((a : α) × β a)) = default := (rfl)
+
 theorem getEntry?_cons [BEq α] {l : List ((a : α) × β a)} {k a : α} {v : β k} :
     getEntry? a (⟨k, v⟩ :: l) = bif k == a then some ⟨k, v⟩ else getEntry? a l := (rfl)
 
@@ -73,6 +90,38 @@ theorem getEntry?_cons_self [BEq α] [ReflBEq α] {l : List ((a : α) × β a)} 
     getEntry? k (⟨k, v⟩ :: l) = some ⟨k, v⟩ :=
   getEntry?_cons_of_true BEq.rfl
 
+theorem getEntryD_cons [BEq α] {l : List ((a : α) × β a)} {k a : α} {v : β k} {fallback : (a : α) × β a} :
+    getEntryD a fallback (⟨k, v⟩ :: l) = bif k == a then ⟨k, v⟩ else getEntryD a fallback l := (rfl)
+
+theorem getEntryD_cons_of_true [BEq α] {l : List ((a : α) × β a)} {k a : α} {v : β k} {fallback : (a : α) × β a}
+    (h : k == a) : getEntryD a fallback (⟨k, v⟩ :: l) = ⟨k, v⟩ := by
+  simp [getEntryD, h]
+
+theorem getEntryD_cons_of_false [BEq α] {l : List ((a : α) × β a)} {k a : α} {v : β k} {fallback : (a : α) × β a}
+    (h : (k == a) = false) : getEntryD a fallback (⟨k, v⟩ :: l) = getEntryD a fallback l := by
+  simp [getEntryD, h]
+
+@[simp]
+theorem getEntryD_cons_self [BEq α] [ReflBEq α] {l : List ((a : α) × β a)} {k : α} {v : β k} {fallback : (a : α) × β a} :
+    getEntryD k fallback (⟨k, v⟩ :: l) = ⟨k, v⟩ :=
+  getEntryD_cons_of_true BEq.rfl
+
+theorem getEntry!_cons [BEq α] {l : List ((a : α) × β a)} {k a : α} {v : β k} [Inhabited ((a : α) × β a)] :
+    getEntry! a (⟨k, v⟩ :: l) = bif k == a then ⟨k, v⟩ else getEntry! a l := (rfl)
+
+theorem getEntry!_cons_of_true [BEq α] {l : List ((a : α) × β a)} {k a : α} {v : β k} [Inhabited ((a : α) × β a)]
+    (h : k == a) : getEntry! a (⟨k, v⟩ :: l) = ⟨k, v⟩ := by
+  simp [getEntry!, h]
+
+theorem getEntry!_cons_of_false [BEq α] {l : List ((a : α) × β a)} {k a : α} {v : β k} [Inhabited ((a : α) × β a)]
+    (h : (k == a) = false) : getEntry! a (⟨k, v⟩ :: l) = getEntry! a l := by
+  simp [getEntry!, h]
+
+@[simp]
+theorem getEntry!_cons_self [BEq α] [ReflBEq α] {l : List ((a : α) × β a)} {k : α} {v : β k} [Inhabited ((a : α) × β a)] :
+    getEntry! k (⟨k, v⟩ :: l) = ⟨k, v⟩ :=
+  getEntry!_cons_of_true BEq.rfl
+
 theorem beq_of_getEntry?_eq_some [BEq α] {l : List ((a : α) × β a)} {a : α} {p : (a : α) × β a}
     (h : getEntry? a l = some p) : p.1 == a := by
   induction l using assoc_induction
@@ -94,6 +143,18 @@ theorem getEntry?_congr [BEq α] [PartialEquivBEq α] {l : List ((a : α) × β 
     · have h₂ : (k == b) = false := BEq.neq_of_neq_of_beq h' h
       rw [getEntry?_cons_of_false h', getEntry?_cons_of_false h₂, ih]
     · rw [getEntry?_cons_of_true h', getEntry?_cons_of_true (BEq.trans h' h)]
+
+theorem getEntryD_eq_getEntry? [BEq α] {l : List ((a : α) × β a)} {a : α} {fallback : (a : α) × β a} :
+    getEntryD a fallback l = (getEntry? a l).getD fallback := by
+  induction l using assoc_induction with
+  | nil => simp [getEntryD, getEntry?]
+  | cons k v t ih => cases h : k == a <;> simp_all [getEntryD, getEntry?]
+
+theorem getEntry!_eq_getEntry? [BEq α] {l : List ((a : α) × β a)} {a : α} [Inhabited ((a : α) × β a)] :
+    getEntry! a l = (getEntry? a l).get! := by
+  induction l using assoc_induction with
+  | nil => rfl
+  | cons k v t ih => cases h : k == a <;> simp_all [getEntry!, getEntry?]
 
 theorem keys_eq_map {l : List ((a : α) × β a)} :
     keys l = l.map (·.1) := by
@@ -483,6 +544,30 @@ theorem getEntry?_eq_some_getEntry [BEq α] {l : List ((a : α) × β a)} {a : �
 theorem getEntry_eq_of_getEntry?_eq_some [BEq α] {l : List ((a : α) × β a)} {k a : α} {v : β k}
     (h : getEntry? a l = some ⟨k, v⟩) {h'} : getEntry a l h' = ⟨k, v⟩ := by
   simp [getEntry, h]
+
+theorem getEntry_cons [BEq α] {l : List ((a : α) × β a)} {k a : α} {v : β k}
+    (h : containsKey a (⟨k, v⟩ :: l)) :
+    getEntry a (⟨k, v⟩ :: l) h =
+      if h' : k == a then
+        ⟨k, v⟩
+      else
+        getEntry a l (containsKey_of_containsKey_cons (k := k) h (Bool.eq_false_iff.2 h')) := by
+  rw [getEntry, Option.get_congr getEntry?_cons]
+  split
+  case _ =>
+    rename_i h
+    simp [h]
+  case _ =>
+    rename_i h
+    simp [h]
+    rw [getEntry]
+
+theorem getEntry_congr [BEq α] [PartialEquivBEq α] {l : List ((a : α) × β a)} {a b : α}
+    (h : a == b) {h₁ h₂} : getEntry a l h₁ = getEntry b l h₂ := by
+  suffices some (getEntry a l h₁) = some (getEntry b l h₂) by
+    injections
+  simp only [← getEntry?_eq_some_getEntry]
+  apply getEntry?_congr h
 
 theorem getEntry_cons_of_beq [BEq α] {l : List ((a : α) × β a)} {k a : α} {v : β k} (h : k == a) :
     getEntry a (⟨k, v⟩ :: l) (containsKey_cons_of_beq (v := v) h) = ⟨k, v⟩ := by
@@ -1622,6 +1707,20 @@ theorem getValueCast_insertEntry [BEq α] [LawfulBEq α] {l : List ((a : α) × 
     getValueCast?_insertEntry]
   simp only [← getValueCast?_eq_some_getValueCast]
 
+theorem getEntry_insertEntry [BEq α] [PartialEquivBEq α] {l : List ((a : α) × β a)} {k a : α}
+    {v : β k} {h} :
+    getEntry a (insertEntry k v l) h = if h' : k == a then ⟨k, v⟩ else getEntry a l (containsKey_of_containsKey_insertEntry h (Bool.eq_false_iff.2 h')) := by
+  suffices some (getEntry a (insertEntry k v l) h) = if h' : (k == a) = true then some ⟨k, v⟩ else some (getEntry a l (containsKey_of_containsKey_insertEntry h (Bool.eq_false_iff.2 h'))) by
+    split <;> (rename_i h; simpa [h] using this)
+  simp only [← getEntry?_eq_some_getEntry]
+  apply getEntry?_insertEntry
+
+theorem beq_of_getEntry_eq [BEq α] [PartialEquivBEq α] {l : List ((a : α) × β a)} {p : ((a : α) × β a)}
+    {k : α} {h₁} (h : getEntry k l h₁ = p) : p.fst == k := by
+  have heq1 : some (getEntry k l h₁) = some p := by simp only [h]
+  rw [← getEntry?_eq_some_getEntry] at heq1
+  exact @beq_of_getEntry?_eq_some α β _ l k p heq1
+
 theorem getValueCast_insertEntry_self [BEq α] [LawfulBEq α] {l : List ((a : α) × β a)} {k : α}
     {v : β k} : getValueCast k (insertEntry k v l) containsKey_insertEntry_self = v := by
   simp [getValueCast_insertEntry]
@@ -2133,6 +2232,14 @@ theorem getEntry?_of_perm [BEq α] [PartialEquivBEq α] {l l' : List ((a : α) �
     exact ((Bool.eq_false_iff.1 hl.2.1).elim (BEq.trans h₁ (BEq.symm h₂))).elim
   next l₁ l₂ l₃ hl₁₂ _ ih₁ ih₂ => exact (ih₁ hl).trans (ih₂ (hl.perm (hl₁₂.symm)))
 
+theorem getEntryD_of_perm [BEq α] [PartialEquivBEq α] {l l' : List ((a : α) × β a)} {a : α} {fallback : (a : α) × β a}
+    (hl : DistinctKeys l) (h : Perm l l') : getEntryD a fallback l = getEntryD a fallback l' := by
+  rw [getEntryD_eq_getEntry?, getEntryD_eq_getEntry?, getEntry?_of_perm hl h]
+
+theorem getEntry!_of_perm [BEq α] [PartialEquivBEq α] {l l' : List ((a : α) × β a)} {a : α} [Inhabited ((a : α) × β a)]
+    (hl : DistinctKeys l) (h : Perm l l') : getEntry! a l = getEntry! a l' := by
+  rw [getEntry!_eq_getEntry?, getEntry!_eq_getEntry?, getEntry?_of_perm hl h]
+
 theorem containsKey_of_perm [BEq α] [PartialEquivBEq α] {l l' : List ((a : α) × β a)} {k : α}
     (h : Perm l l') : containsKey k l = containsKey k l' := by
   induction h
@@ -2152,6 +2259,12 @@ theorem getValueCast_of_perm [BEq α] [LawfulBEq α] {l l' : List ((a : α) × �
     getValueCast a l h' = getValueCast a l' ((containsKey_of_perm h).symm.trans h') := by
   rw [← Option.some_inj, ← getValueCast?_eq_some_getValueCast, ← getValueCast?_eq_some_getValueCast,
     getValueCast?_of_perm hl h]
+
+theorem getEntry_of_perm [BEq α] [PartialEquivBEq α] {l l' : List ((a : α) × β a)} {a : α} {h'} (hl : DistinctKeys l) (h : Perm l l') : getEntry a l h' = getEntry a l' ((containsKey_of_perm h).symm.trans h') := by
+  suffices some (getEntry a l h') = some (getEntry a l' ((containsKey_of_perm h).symm.trans h')) by injections
+  rw [← getEntry?_eq_some_getEntry, ← getEntry?_eq_some_getEntry]
+  apply getEntry?_of_perm hl h
+
 
 theorem getValueCast!_of_perm [BEq α] [LawfulBEq α] {l l' : List ((a : α) × β a)} {a : α}
     [Inhabited (β a)] (hl : DistinctKeys l) (h : Perm l l') :
@@ -2328,6 +2441,14 @@ theorem getEntry?_append_of_containsKey_eq_false [BEq α] {l l' : List ((a : α)
     (h : containsKey a l' = false) : getEntry? a (l ++ l') = getEntry? a l := by
   rw [getEntry?_append, getEntry?_eq_none.2 h, Option.or_none]
 
+theorem getEntryD_append_of_containsKey_eq_false [BEq α] {l l' : List ((a : α) × β a)} {a : α} {fallback : (a : α) × β a}
+    (h : containsKey a l' = false) : getEntryD a fallback (l ++ l') = getEntryD a fallback l := by
+  simp [getEntryD_eq_getEntry?, getEntry?_append_of_containsKey_eq_false h]
+
+theorem getEntry!_append_of_containsKey_eq_false [BEq α] {l l' : List ((a : α) × β a)} {a : α} [Inhabited ((a : α) × β a)]
+    (h : containsKey a l' = false) : getEntry! a (l ++ l') = getEntry! a l := by
+  simp [getEntry!_eq_getEntry?, getEntry?_append_of_containsKey_eq_false h]
+
 @[simp]
 theorem containsKey_append [BEq α] {l l' : List ((a : α) × β a)} {a : α} :
     containsKey a (l ++ l') = (containsKey a l || containsKey a l') := by
@@ -2376,6 +2497,12 @@ theorem getValueCast_append_of_containsKey_eq_false [BEq α] [LawfulBEq α]
       getValueCast a l ((containsKey_append_of_not_contains_right hl').symm.trans h) := by
   rw [← Option.some_inj, ← getValueCast?_eq_some_getValueCast, ← getValueCast?_eq_some_getValueCast,
     getValueCast?_append_of_containsKey_eq_false hl']
+
+theorem getEntry_append_of_containsKey_eq_false [BEq α] {l l' : List ((a : α) × β a)} {a : α} {h} (hl' : containsKey a l' = false) : getEntry a (l ++ l') h = getEntry a l ((containsKey_append_of_not_contains_right hl').symm.trans h) := by
+  suffices some (getEntry a (l ++ l') h) = some (getEntry a l ((containsKey_append_of_not_contains_right hl').symm.trans h)) by
+    injections
+  simp only [← getEntry?_eq_some_getEntry]
+  apply getEntry?_append_of_containsKey_eq_false hl'
 
 theorem getKey?_append_of_containsKey_eq_false [BEq α] [PartialEquivBEq α]
     {l l' : List ((a : α) × β a)} {a : α} (hl' : containsKey a l' = false) :
